iodiv/DivFreeTauDM.Test.fst
@@ -1,0 +1,32 @@
+module DivFreeTauDM.Test
+
+open FStar.List.Tot
+open FStar.Tactics
+
+open DivFree
+open DivFreeTauSpec
+open DivFreeTauDM
+
+open IIOSig
+open IIOSigSpec
+
+open DivFree.Test
+open DivFreeTauSpec.Test
+
+let th #a = theta #a #io_sig iodiv_act
+
+
+let test1 (fd:file_descr) : Lemma (th (body1 fd) `ile` ibody1 fd) = ()
+
+
+let test2 (fd:file_descr) =
+//  pre1_inv1 fd;
+  let body' = lift_body #file_descr (ibody1 fd) #unit in
+//  let body_inv = repeat_body_inv #unit (fun _ -> pre1 fd) (inv1 fd) in
+//  repeat_inv_proof #unit (fun _ -> (pre1 fd)) (inv1 fd) () ;
+//  i_iter_mono (fun _ -> repeat_body_inv (fun _ -> (pre1 fd)) (inv1 fd) ()) (repeat_body_inv (fun _ -> (pre1 fd)) (inv1 fd)) () ;
+
+  test1 fd;
+  assume (th (loop1 fd) `ile` i_iter body' ());
+  itest1 fd;
+  assert (th (loop1 fd) `ile` iloop1 fd)
